Infra/LengthEq.v
@@ -52,6 +52,7 @@ Ltac length_equify :=
               eapply length_length_eq in H
           end).
 
+Hint Resolve length_length_eq length_eq_length : len.
 
 
 
